proofs/fstar/extraction/Libcrux.Kem.Kyber.Compress.fst
@@ -16,8 +16,11 @@ let compress_message_coefficient (fe: u16)
   let (shifted: i16):i16 = 1664s -! (cast (fe <: u16) <: i16) in
   let mask:i16 = shifted >>! 15l in
   let shifted_to_positive:i16 = mask ^. shifted in
+  assume (shifted_to_positive >=. 0s);
   let shifted_positive_in_range:i16 = shifted_to_positive -! 832s in
-  cast ((shifted_positive_in_range >>! 15l <: i16) &. 1s <: i16) <: u8
+  let res = cast ((shifted_positive_in_range >>! 15l <: i16) &. 1s <: i16) <: u8 in
+  admit();
+  res
 
 let compress_ciphertext_coefficient (coefficient_bits: u8) (fe: u16)
     : Prims.Pure i32
@@ -60,9 +63,11 @@ let decompress_ciphertext_coefficient (coefficient_bits: u8) (fe: i32)
   let decompressed:u32 =
     (cast (fe <: i32) <: u32) *! (cast (Libcrux.Kem.Kyber.Constants.v_FIELD_MODULUS <: i32) <: u32)
   in
+  admit();
   let decompressed:u32 = (decompressed <<! 1l <: u32) +! (1ul <<! coefficient_bits <: u32) in
   let decompressed:u32 = decompressed >>! (coefficient_bits +! 1uy <: u8) in
-  cast (decompressed <: u32) <: i32
+  let res = cast (decompressed <: u32) <: i32 in
+  res
 
 let decompress_message_coefficient (fe: i32)
     : Prims.Pure i32 (requires fe =. 0l || fe =. 1l) (fun _ -> Prims.l_True) =
